add total map VSTs for all ordered semantics

core/TotalMapSimulations.v
@@ -4,10 +4,13 @@ Import ListNotations.
 Require Import StructTact.StructTactics.
 Require Import StructTact.Util.
 Require Import Verdi.Net.
+Require Import Verdi.DynamicNetLemmas.
 
 Local Arguments update {_} {_} _ _ _ _ _ : simpl never.
 
 Require Import FunctionalExtensionality.
+Require Import Sorting.Permutation.
+Require Import Sumbool.
 
 Require Import mathcomp.ssreflect.ssreflect.
 
@@ -88,6 +91,34 @@ Class FailureParamsTotalMapCongruency
   (B : BaseParamsTotalMap B0 B1) :=
   {
     tot_reboot_eq : forall d, tot_map_data (reboot d) = reboot (tot_map_data d)
+  }.
+
+Class NameOverlayParamsTotalMapCongruency
+  (B0 : BaseParams) (B1 : BaseParams)
+  (P0 : MultiParams B0) (P1 : MultiParams B1)
+  (O0 : NameOverlayParams P0) (O1 : NameOverlayParams P1)
+  (N : MultiParamsNameTotalMap P0 P1) :=
+  {
+    tot_adjacent_to_fst_snd : forall n n',
+      adjacent_to n n' <-> adjacent_to (tot_map_name n) (tot_map_name n')
+  }.
+
+Class FailMsgParamsTotalMapCongruency
+  (B0 : BaseParams) (B1 : BaseParams)
+  (P0 : MultiParams B0) (P1 : MultiParams B1)
+  (F0 : FailMsgParams P0) (F1 : FailMsgParams P1)
+  (P : MultiParamsMsgTotalMap P0 P1) :=
+  {
+    tot_fail_msg_fst_snd : msg_fail = tot_map_msg msg_fail
+  }.
+
+Class NewMsgParamsTotalMapCongruency
+  (B0 : BaseParams) (B1 : BaseParams)
+  (P0 : MultiParams B0) (P1 : MultiParams B1)
+  (N0 : NewMsgParams P0) (N1 : NewMsgParams P1)
+  (P : MultiParamsMsgTotalMap P0 P1) :=
+  {
+    tot_new_msg_fst_snd : msg_new = tot_map_msg msg_new
   }.
 
 Section TotalMapBijective.
@@ -831,6 +862,860 @@ invcs H_step.
         end.
         by find_rewrite_lem tot_map_name_inv_inverse.
     by rewrite H_eq_sw.
+Qed.
+
+Lemma nodup_to_map_name :
+  forall ns, NoDup ns ->
+        NoDup (map tot_map_name ns).
+Proof.
+elim => /=; first by move => H_nd; exact: NoDup_nil.
+move => n ns IH H_nd.
+inversion H_nd.
+find_apply_lem_hyp IH.
+by apply NoDup_cons; first exact: not_in_failed_not_in.  
+Qed.
+
+Lemma permutation_nodes :
+  Permutation nodes (map tot_map_name nodes).
+Proof.
+apply: NoDup_Permutation; last split.
+- exact: no_dup_nodes.
+- apply nodup_to_map_name.
+  exact: no_dup_nodes.
+- move => H_in.
+  set x' := tot_map_name_inv x.
+  have H_in' := all_names_nodes x'. 
+  apply in_split in H_in'.
+  move: H_in' => [ns1 [ns2 H_eq]].
+  rewrite H_eq map_app /= /x'.
+  apply in_or_app.
+  right; left.
+  by rewrite tot_map_name_inverse_inv.
+- move => H_in.
+  exact: all_names_nodes.
+Qed.
+
+Context {overlay_fst : NameOverlayParams multi_fst}.
+Context {overlay_snd : NameOverlayParams multi_snd}.
+Context {overlay_map_congr : NameOverlayParamsTotalMapCongruency overlay_fst overlay_snd name_map}.
+
+Lemma tot_map_in_snd :
+forall h m ns nm,
+   In nm
+     (map
+        (fun nm0 : name * msg =>
+         (tot_map_name (fst nm0), tot_map_msg (snd nm0)))
+        (map2snd m (filter_rel adjacent_to_dec h ns))) ->
+   snd nm = tot_map_msg m.
+Proof.
+move => h m.
+elim => //=.
+move => n ns IH.
+case (adjacent_to_dec _ _) => H_dec /=.
+  case => n' m' H_in.
+  case: H_in => H_in.
+    by inversion H_in.
+  exact: IH.
+exact: IH.
+Qed.
+
+Lemma tot_map_in_in :
+  forall n m l,
+  (forall nm, In nm l -> snd nm = m) ->
+  ~ In (n, m) l ->
+  ~ In (tot_map_name n, tot_map_msg m) (map (fun nm : name * msg => (tot_map_name (fst nm), tot_map_msg (snd nm))) l).
+Proof.
+move => n m.
+elim => //=.
+case => /= n' m' l IH H_eq H_in.
+move => H_in'.
+case: H_in' => H_in'.
+  inversion H_in'.
+  have H_nm := H_eq (n', m').
+  rewrite /= in H_nm.
+  case: H_in.
+  left.
+  apply tot_map_name_injective in H0.
+  rewrite H0.
+  rewrite H_nm //.
+  by left.
+contradict H_in'.
+apply: IH.
+  move => nm H_in_nm.
+  apply: H_eq.
+  by right.
+move => H_in_nm.
+case: H_in.
+by right.
+Qed.
+
+Lemma msg_in_map :
+  forall m l n m',
+    (forall nm, In nm l -> snd nm = m) ->
+    In (tot_map_name n, tot_map_msg m') (map (fun nm : name * msg => (tot_map_name (fst nm), tot_map_msg (snd nm))) l) ->
+    tot_map_msg m' = tot_map_msg m.
+Proof.
+move => m.
+elim => //=.
+case => /= n m' l IH n' m0 H_in H_in_map.
+have H_in_f := H_in (n, m').
+rewrite /= in H_in_f.
+case: H_in_map => H_in_map.
+  inversion H_in_map.
+  rewrite H_in_f //.
+  by left.
+move: H_in_map.
+apply: IH.
+move => nm H_in'.
+apply: H_in.
+by right.
+Qed.
+
+Lemma nodup_tot_map :
+  forall m nms,
+  (forall nm, In nm nms -> snd nm = m) ->
+  NoDup nms ->
+  NoDup (map (fun nm : name * msg => (tot_map_name (fst nm), tot_map_msg (snd nm))) nms).
+Proof.
+move => m'.
+elim => /=.
+  move => H_fail H_nd.
+  exact: NoDup_nil.
+case => n m l IH H_fail H_nd.
+inversion H_nd.
+rewrite /=.
+apply NoDup_cons.
+  have H_f := H_fail (n, m).
+  rewrite /= in H_f.
+  move => H_in.
+   have H_inf := @msg_in_map m' _ _ _ _ H_in.
+   rewrite H_inf in H_in.
+     contradict H_in.
+     apply tot_map_in_in.
+       move => nm H_in_nm.
+       apply: H_fail.
+       by right.
+     rewrite H_f // in H1.
+     by left.
+   move => nm H_in_f.
+   apply: H_fail.
+   by right.
+apply: IH => //.
+move => nm H_in_nm.
+apply: H_fail.
+by right.
+Qed.
+
+Lemma in_tot_map_name :
+forall m l n,
+  (forall nm, In nm l -> snd nm = m) ->
+  In (n, tot_map_msg m) (map (fun nm : name * msg => (tot_map_name (fst nm), tot_map_msg (snd nm))) l) ->
+  In (tot_map_name_inv n, m) l.
+Proof.
+move => m.
+elim => //=.
+case => /= n m' l IH n' H_in H_in'.
+case: H_in' => H_in'.
+  inversion H_in'.
+  rewrite tot_map_name_inv_inverse.
+  have H_nm := H_in (n, m').
+  rewrite -H_nm /=; first by left.
+  by left.
+right.
+apply: IH => //.
+move => nm H_inn.
+apply: H_in.
+by right.
+Qed.
+
+Lemma in_map_pair_adjacent_to :
+  forall (m : @msg _ multi_fst) ns failed h n,
+    In (tot_map_name_inv n, m) (map2snd m (filter_rel adjacent_to_dec h (remove_all name_eq_dec failed ns))) ->
+    In (tot_map_name_inv n) (filter_rel adjacent_to_dec h (remove_all name_eq_dec failed ns)).
+Proof.
+move => m.
+elim => //= [|n l IH] failed h n'; first by rewrite remove_all_nil.
+have H_cn := remove_all_cons name_eq_dec failed n l.
+break_or_hyp; break_and; find_rewrite; first exact: IH.
+rewrite /=.
+case (adjacent_to_dec _ _) => H_dec' /=.
+  move => H_in.
+  case: H_in => H_in.
+    inversion H_in.
+    by left.
+  right.
+  exact: IH.
+exact: IH.
+Qed.
+
+Lemma in_adjacent_exclude_in_exlude :
+  forall ns failed n h,
+    In (tot_map_name_inv n) (filter_rel adjacent_to_dec h (remove_all name_eq_dec failed ns)) ->
+    In (tot_map_name_inv n) (remove_all name_eq_dec failed ns) /\ adjacent_to h (tot_map_name_inv n).
+Proof.
+elim => [|n l IH] failed n' h; first by rewrite remove_all_nil.
+have H_cn := remove_all_cons name_eq_dec failed n l.
+break_or_hyp; break_and; find_rewrite; first exact: IH.
+rewrite /=.
+case (adjacent_to_dec _ _) => /= H_dec'.
+  move => H_in.
+  case: H_in => H_in.
+    rewrite {1}H_in -{4}H_in.
+    split => //.
+    by left.
+  apply IH in H_in.
+  move: H_in => [H_eq H_in].
+  split => //.
+  by right.
+move => H_in.
+apply IH in H_in.
+move: H_in => [H_eq H_in].
+split => //.
+by right.
+Qed.
+
+Lemma in_failed_exclude :
+  forall ns failed n,
+    In (tot_map_name_inv n) (remove_all name_eq_dec failed ns) ->
+    ~ In (tot_map_name_inv n) failed /\ In (tot_map_name_inv n) ns.
+Proof.
+elim => [|n ns IH] failed n'; first by rewrite remove_all_nil.
+have H_cn := remove_all_cons name_eq_dec failed n ns.
+break_or_hyp; break_and; find_rewrite.
+  move => H_in.
+  apply IH in H_in.
+  move: H_in => [H_in H_in'].
+  split => //.
+  by right.
+move => H_in.
+case: H_in => H_in.
+  rewrite -{1}H_in {2}H_in.
+  split => //.
+  by left.
+apply IH in H_in.
+move: H_in => [H_in H_in'].
+split => //.
+by right.
+Qed.
+
+Lemma in_in_adj_map_pair :
+  forall (m : msg) ns failed n h,
+    In n ns ->
+    ~ In n (map tot_map_name failed) ->
+    adjacent_to h n ->
+    In (n, m)
+     (map2snd m
+        (filter_rel adjacent_to_dec h
+           (remove_all name_eq_dec (map tot_map_name failed) ns))).
+Proof.
+move => m.
+elim => //=.
+move => n ns IH failed n' h.
+set mfailed := map _ failed.
+move => H_in H_in' H_adj.
+have H_cn := remove_all_cons name_eq_dec mfailed n ns.
+break_or_hyp; break_and; find_rewrite.
+  break_or_hyp => //.
+  exact: IH.
+case: H_in => H_in.
+  rewrite H_in.
+  rewrite /=.
+  case (adjacent_to_dec _ _) => H_dec' //.
+  rewrite /=.
+  by left.
+rewrite /=.
+case (adjacent_to_dec _ _) => H_dec'.
+  rewrite /=.
+  right.
+  exact: IH.
+exact: IH.
+Qed.
+
+Lemma in_exclude_not_in_failed_map :
+  forall ns n failed,
+  In n (remove_all name_eq_dec (map tot_map_name failed) ns) ->
+  ~ In n (map tot_map_name failed) /\ In n ns.
+Proof.
+elim => [|n ns IH] n' failed; first by rewrite remove_all_nil.
+set mfailed := map _ failed.
+have H_cn := remove_all_cons name_eq_dec mfailed n ns.
+break_or_hyp; break_and; find_rewrite.
+  move => H_in.
+  apply IH in H_in.
+  move: H_in => [H_nin H_in].
+  split => //.
+  by right.
+rewrite /=.
+move => H_in.
+case: H_in => H_in.
+  rewrite H_in.
+  subst.
+  split => //.
+  by left.
+apply IH in H_in.
+move: H_in => [H_nin H_in].
+split => //.
+by right.
+Qed.
+
+Lemma not_in_map_not_in_failed :
+  forall failed n,
+    ~ In n (map tot_map_name failed) ->
+    ~ In (tot_map_name_inv n) failed.
+Proof.
+elim => //=.
+move => n ns IH n' H_in H_in'.
+case: H_in' => H_in'.
+  case: H_in.
+  left.
+  by rewrite H_in' tot_map_name_inverse_inv.
+contradict H_in'.
+apply: IH.
+move => H_in'.
+case: H_in.
+by right.
+Qed.
+
+Lemma in_tot_map_msg :
+  forall m l n,
+    (forall nm, In nm l -> snd nm = m) ->
+    In (tot_map_name_inv n, m) l ->
+    In (n, tot_map_msg m) (map (fun nm : name * msg => (tot_map_name (fst nm), tot_map_msg (snd nm))) l).
+Proof.
+move => m.
+elim => //=.
+case => n m' /= l IH n' H_in H_in'.
+case: H_in' => H_in'.
+  inversion H_in'.
+  left.
+  by rewrite tot_map_name_inverse_inv.
+right.
+apply: IH => //.
+move => nm H_inn.
+apply: H_in.
+by right.
+Qed.
+
+Lemma adjacent_in_in_msg :
+  forall (m : @msg base_fst multi_fst) ns n h,
+    adjacent_to h (tot_map_name_inv n) ->
+    In (tot_map_name_inv n) ns ->
+    In (tot_map_name_inv n, m) (map2snd m (filter_rel adjacent_to_dec h ns)).
+Proof.
+move => m.
+elim => //=.
+move => n ns IH n' h H_adj H_in.
+case (adjacent_to_dec _ _) => H_dec; case: H_in => H_in.
+- rewrite /=.
+  left.
+  by rewrite H_in.
+- rewrite /=.
+  right.
+  exact: IH.
+- by rewrite H_in in H_dec.
+- exact: IH.
+Qed.
+
+Lemma not_in_failed_in_exclude :
+  forall ns n failed,
+  ~ In (tot_map_name_inv n) failed ->
+  In (tot_map_name_inv n) ns ->
+  In (tot_map_name_inv n) (remove_all name_eq_dec failed ns).
+Proof.
+elim => //=.
+move => n ns IH n' failed H_in H_in'.
+have H_cn := remove_all_cons name_eq_dec failed n ns.
+break_or_hyp; break_and; find_rewrite; break_or_hyp => //=. 
+- exact: IH.
+- by left.
+- right; exact: IH.
+Qed.
+
+Lemma tot_map_name_in : 
+  forall ns n,
+    In (tot_map_name n) (map tot_map_name ns) ->
+    In n ns.
+Proof.
+elim => //=.
+move => n' ns IH n H_in.
+case: H_in => H_in.
+  left.
+  exact: tot_map_name_injective.
+right.
+exact: IH.
+Qed.
+
+Lemma nodup_perm_map_map_pair_perm :
+  forall h m failed ns ns',
+  NoDup ns ->
+  Permutation (map tot_map_name ns) ns' ->
+  Permutation 
+    (map (fun nm : name * msg => (tot_map_name (fst nm), tot_map_msg (snd nm))) (map2snd m (filter_rel adjacent_to_dec h (remove_all name_eq_dec failed ns)))) 
+    (map2snd (tot_map_msg m) (filter_rel adjacent_to_dec (tot_map_name h) (remove_all name_eq_dec (map tot_map_name failed) ns'))).
+Proof.
+move => h m failed ns ns' H_nd H_pm.
+apply NoDup_Permutation; last split.
+- apply (@nodup_tot_map m); first exact: in_map2snd_snd.
+  apply NoDup_map2snd.
+  by apply NoDup_remove_all.
+- apply NoDup_map2snd.
+  apply NoDup_remove_all.
+  move: H_pm.
+  apply: NoDup_Permutation_NoDup.
+  exact: nodup_to_map_name.
+- case: x => n m' H_in.
+  have H_eq := tot_map_in_snd _ _ _ _ H_in.
+  rewrite /= in H_eq.
+  rewrite H_eq in H_in.
+  rewrite H_eq {H_eq}.
+  apply in_tot_map_name in H_in.
+    apply in_map2snd_related_in in H_in.
+    move: H_in => [H_adj H_in].
+    apply in_failed_exclude in H_in.
+    move: H_in => [H_in H_in'].
+    have H_nin: ~ In n (map tot_map_name failed).
+      rewrite -(tot_map_name_inverse_inv n).
+      exact: not_in_failed_not_in.
+    apply tot_adjacent_to_fst_snd in H_adj.
+    rewrite tot_map_name_inverse_inv in H_adj.
+    have H_inn: In n ns'.
+      apply (Permutation_in n) in H_pm => //.
+      rewrite -(tot_map_name_inverse_inv n).
+      exact: in_failed_in.
+    exact: in_in_adj_map_pair.
+  exact: in_map2snd_snd.
+- case: x => n m' H_in.
+  have H_eq := in_map2snd_snd _ _ adjacent_to adjacent_to_dec _ _ _ _ H_in.
+  rewrite /= in H_eq.
+  rewrite H_eq.
+  rewrite H_eq in H_in.
+  apply in_map2snd_related_in in H_in.
+  move: H_in => [H_adj H_in].
+  rewrite -(tot_map_name_inverse_inv n) in H_adj.
+  apply tot_adjacent_to_fst_snd in H_adj.
+  apply in_exclude_not_in_failed_map in H_in.
+  move: H_in => [H_in_f H_in].
+  apply not_in_map_not_in_failed in H_in_f.
+  have H_in_n: In (tot_map_name_inv n) ns.
+    apply Permutation_sym in H_pm.
+    apply (Permutation_in n) in H_pm => //.
+    apply: tot_map_name_in.
+    by rewrite tot_map_name_inverse_inv.
+  apply in_tot_map_msg; first by move => nm; apply in_map2snd_snd.
+  apply: adjacent_in_in_msg => //.
+  exact: not_in_failed_in_exclude.
+Qed.
+
+Lemma map_map_pair_eq :
+  forall h m failed,
+  Permutation 
+    (map (fun nm : name * msg => (tot_map_name (fst nm), tot_map_msg (snd nm))) (map2snd m (filter_rel adjacent_to_dec h (remove_all name_eq_dec failed nodes)))) 
+    (map2snd (tot_map_msg m) (filter_rel adjacent_to_dec (tot_map_name h) (remove_all name_eq_dec (map tot_map_name failed) nodes))).
+Proof.
+move => h m failed.
+apply nodup_perm_map_map_pair_perm; first exact: no_dup_nodes.
+apply Permutation_sym.
+exact: permutation_nodes.
+Qed.
+
+Context {fail_msg_fst : FailMsgParams multi_fst}.
+Context {fail_msg_snd : FailMsgParams multi_snd}.
+Context {fail_msg_map_congr : FailMsgParamsTotalMapCongruency fail_msg_fst fail_msg_snd msg_map}.
+
+Lemma map_msg_fail_eq_nodup :
+  forall h failed ns ns',
+  NoDup ns ->
+  Permutation (map tot_map_name ns) ns' ->
+   Permutation 
+    (map (fun nm : name * msg => (tot_map_name (fst nm), tot_map_msg (snd nm))) (map2snd msg_fail (filter_rel adjacent_to_dec h (remove_all name_eq_dec failed ns)))) 
+    (map2snd msg_fail (filter_rel adjacent_to_dec (tot_map_name h) (remove_all name_eq_dec (map tot_map_name failed) ns'))).
+Proof.
+move => h failed.
+rewrite tot_fail_msg_fst_snd.
+exact: nodup_perm_map_map_pair_perm.
+Qed.
+
+Lemma map_msg_fail_eq :
+  forall h failed,
+   Permutation 
+    (map (fun nm : name * msg => (tot_map_name (fst nm), tot_map_msg (snd nm))) (map2snd msg_fail (filter_rel adjacent_to_dec h (remove_all name_eq_dec failed nodes)))) 
+    (map2snd msg_fail (filter_rel adjacent_to_dec (tot_map_name h) (remove_all name_eq_dec (map tot_map_name failed) nodes))).
+Proof.
+move => h failed.
+rewrite tot_fail_msg_fst_snd.
+exact: map_map_pair_eq.
+Qed.
+
+Definition tot_map_onet (onet : @ordered_network _ multi_fst) : @ordered_network _ multi_snd :=
+  {| onwPackets := fun src dst => map tot_map_msg (onet.(onwPackets) (tot_map_name_inv src) (tot_map_name_inv dst)) ;
+     onwState := fun n => tot_map_data (onet.(onwState) (tot_map_name_inv n)) |}.
+
+Lemma map_msg_update2 : 
+  forall f ms to from,
+    (fun src dst => map tot_map_msg (update2 name_eq_dec f from to ms (tot_map_name_inv src) (tot_map_name_inv dst))) =
+    update2 name_eq_dec (fun src0 dst0 : name => map tot_map_msg (f (tot_map_name_inv src0) (tot_map_name_inv dst0)))
+        (tot_map_name from) (tot_map_name to) (map tot_map_msg ms).
+Proof.
+move => f ms to from.
+apply functional_extensionality => src.
+apply functional_extensionality => dst.
+rewrite /update2 /=.
+case (sumbool_and _ _ _ _) => H_dec; case (sumbool_and _ _ _ _) => H_dec' //.
+  move: H_dec => [H_eq H_eq'].
+  case: H_dec' => H_dec'.
+    rewrite H_eq in H_dec'.
+    by rewrite tot_map_name_inverse_inv in H_dec'.
+  rewrite H_eq' in H_dec'.
+  by rewrite tot_map_name_inverse_inv in H_dec'.
+move: H_dec' => [H_eq H_eq'].
+case: H_dec => H_dec.
+  rewrite -H_eq in H_dec.
+  by rewrite tot_map_name_inv_inverse in H_dec.
+rewrite -H_eq' in H_dec.
+by rewrite tot_map_name_inv_inverse in H_dec.
+Qed.
+
+Lemma collate_tot_map_eq :
+  forall f h l,
+    (fun src dst => map tot_map_msg (collate name_eq_dec h f l (tot_map_name_inv src) (tot_map_name_inv dst))) =
+    collate name_eq_dec (tot_map_name h) (fun src dst => map tot_map_msg (f (tot_map_name_inv src) (tot_map_name_inv dst))) (tot_map_name_msgs l).
+Proof.
+move => f h l.
+elim: l h f => //.
+case => n m l IH h f.
+rewrite /= IH /=.
+rewrite 2!tot_map_name_inv_inverse /=.
+set f1 := fun _ _ => _.
+set f2 := update2 _ _ _ _ _.
+have H_eq_f: f1 = f2.
+  rewrite /f1 /f2 {f1 f2}.
+  have H_eq := map_msg_update2 f (f h n ++ [m]) n h.
+  rewrite map_app in H_eq.
+  by rewrite H_eq.
+by rewrite H_eq_f.
+Qed.
+
+Lemma collate_tot_map_update2_eq :
+  forall f from to ms l,
+    (fun src dst => map tot_map_msg
+            (collate name_eq_dec to (update2 name_eq_dec f from to ms) l
+               (tot_map_name_inv src) (tot_map_name_inv dst))) =
+    collate name_eq_dec (tot_map_name to)
+            (update2 name_eq_dec
+               (fun src dst : name =>
+                map tot_map_msg
+                  (f (tot_map_name_inv src) (tot_map_name_inv dst))) (tot_map_name from)
+               (tot_map_name to) (map tot_map_msg ms)) (tot_map_name_msgs l).
+Proof.
+move => f from to ms l.
+rewrite -map_msg_update2.
+by rewrite collate_tot_map_eq.
+Qed.
+
+Definition tot_map_trace (e : @name _ multi_fst * (@input base_fst + (@output base_fst))) :=
+match e with
+| (n, inl i) => (tot_map_name n, inl (tot_map_input i))
+| (n, inr o) => (tot_map_name n, inr (tot_map_output o))
+end.
+
+Lemma map_tot_map_trace_eq :
+  forall out to,
+    map tot_map_trace (map2fst to (map inr out)) =
+    map2fst (tot_map_name to) (map inr (map tot_map_output out)).
+elim => //=.
+move => o out IH to.
+by rewrite IH.
+Qed.
+
+Theorem step_ordered_failure_tot_mapped_simulation_1 :
+  forall net net' failed failed' tr,
+    @step_ordered_failure _ _ overlay_fst fail_msg_fst (failed, net) (failed', net') tr ->
+    @step_ordered_failure _ _ overlay_snd fail_msg_snd (map tot_map_name failed, tot_map_onet net) (map tot_map_name failed', tot_map_onet net') (map tot_map_trace tr).
+Proof.
+move => net net' failed failed' tr H_step.
+invcs H_step.
+- rewrite /tot_map_onet /=.
+  apply (@StepOrderedFailure_deliver _ _ _ _ _ _ _ _ (tot_map_msg m) (map tot_map_msg ms) (map tot_map_output out) (tot_map_data d) (tot_map_name_msgs l) (tot_map_name from) (tot_map_name to)).
+  * by rewrite /tot_map_net /= 2!tot_map_name_inv_inverse /= H3.
+  * exact: not_in_failed_not_in.
+  * rewrite /= tot_map_name_inv_inverse -tot_net_handlers_eq /tot_mapped_net_handlers /=.
+    repeat break_let.
+    by find_inversion.
+  * by rewrite /= tot_map_update_eq collate_tot_map_update2_eq.
+  * by rewrite map_tot_map_trace_eq.
+- rewrite /tot_map_onet /=.
+  apply (@StepOrderedFailure_input _ _ _ _ (tot_map_name h) _ _ _ _ (map tot_map_output out) (tot_map_input inp) (tot_map_data d) (tot_map_name_msgs l)).
+  * exact: not_in_failed_not_in.
+  * rewrite /= tot_map_name_inv_inverse -tot_input_handlers_eq /tot_mapped_input_handlers.
+    repeat break_let.
+    by find_inversion.
+  * by rewrite /= /tot_map_onet /= tot_map_update_eq collate_tot_map_eq.
+  * by rewrite map_tot_map_trace_eq.
+- rewrite /tot_map_onet /=.
+  set l := map2snd _ _.
+  have H_nd: NoDup (map fst (tot_map_name_msgs l)).
+    rewrite /tot_map_name_msgs /=.
+    rewrite /l {l} /=.
+    eapply NoDup_map_snd_fst.
+      apply (@nodup_tot_map msg_fail); first exact: in_map2snd_snd.
+      apply NoDup_map2snd.
+      apply NoDup_remove_all.
+      exact: no_dup_nodes.
+    move => nm nm' H_in H_in'.
+    have H_fail := tot_map_in_snd _ _ _ _ H_in.
+    have H_fail' := tot_map_in_snd _ _ _ _ H_in'.
+    by rewrite H_fail H_fail'.
+  have H_pm := map_msg_fail_eq h failed.
+  have H_eq := NoDup_Permutation_collate_eq  _ _ name_eq_dec _ _ _ _ H_nd H_pm.
+  rewrite /l /tot_map_name_msgs in H_eq.
+  apply: StepOrderedFailure_fail.
+  * exact: not_in_failed_not_in.
+  * rewrite /=.
+    rewrite /l collate_tot_map_eq /tot_map_name_msgs.
+    by rewrite H_eq.
+Qed.
+
+Corollary step_ordered_failure_tot_mapped_simulation_star_1 :
+  forall net failed tr,
+    @step_ordered_failure_star _ _ overlay_fst fail_msg_fst step_ordered_failure_init (failed, net) tr ->
+    @step_ordered_failure_star _ _ overlay_snd fail_msg_snd step_ordered_failure_init (map tot_map_name failed, tot_map_onet net) (map tot_map_trace tr).
+Proof.
+move => net failed tr H_step.
+remember step_ordered_failure_init as y in *.
+change failed with (fst (failed, net)).
+change net with (snd (failed, net)) at 2.
+move: Heqy.
+induction H_step using refl_trans_1n_trace_n1_ind => H_init /=.
+  rewrite H_init /step_ordered_failure_init /= /step_ordered_failure_init /tot_map_onet /= tot_init_handlers_fun_eq.
+  exact: RT1nTBase.
+concludes.
+repeat find_rewrite.
+destruct x'.
+destruct x''.
+rewrite /=.
+find_apply_lem_hyp step_ordered_failure_tot_mapped_simulation_1.
+rewrite map_app.
+match goal with
+| H : step_ordered_failure_star _ _ _ |- _ => apply: (refl_trans_1n_trace_trans H)
+end.
+rewrite (app_nil_end (map tot_map_trace _)).
+apply (@RT1nTStep _ _ _ _ (map tot_map_name l0, tot_map_onet o0)) => //.
+exact: RT1nTBase.
+Qed.
+
+Context {new_msg_fst : NewMsgParams multi_fst}.
+Context {new_msg_snd : NewMsgParams multi_snd}.
+Context {new_msg_map_congr : NewMsgParamsTotalMapCongruency new_msg_fst new_msg_snd msg_map}.
+
+Definition tot_map_odnet (net : @ordered_dynamic_network _ multi_fst) : @ordered_dynamic_network _ multi_snd :=
+  {| odnwNodes := map tot_map_name net.(odnwNodes) ;
+     odnwPackets := fun src dst => map tot_map_msg (net.(odnwPackets) (tot_map_name_inv src) (tot_map_name_inv dst)) ;
+     odnwState := fun n => 
+                   match net.(odnwState) (tot_map_name_inv n) with
+                   | None => None
+                   | Some d => Some (tot_map_data d)
+                   end |}.
+
+Lemma collate_ls_tot_map_eq :
+  forall ns f h m,
+    (fun src dst => map tot_map_msg (collate_ls name_eq_dec ns f h m (tot_map_name_inv src) (tot_map_name_inv dst))) =
+    collate_ls name_eq_dec (map tot_map_name ns) (fun src dst => map tot_map_msg (f (tot_map_name_inv src) (tot_map_name_inv dst))) (tot_map_name h) (tot_map_msg m).
+Proof.
+elim => //=.
+move => n ns IH f h m.
+rewrite /= IH /=.
+rewrite 2!tot_map_name_inv_inverse /=.
+set f1 := fun _ _ => _.
+set f2 := update2 _ _ _ _ _.
+have H_eq_f: f1 = f2.
+  rewrite /f1 /f2 {f1 f2}.
+  have H_eq := map_msg_update2 f (f n h ++ [m]) h n.
+  rewrite map_app in H_eq.
+  by rewrite H_eq.
+by rewrite H_eq_f.
+Qed.
+
+Lemma collate_ls_tot_map_update2_eq :
+  forall ns f h m from to ms,
+    (fun src dst => map tot_map_msg
+            (collate_ls name_eq_dec ns (update2 name_eq_dec f from to ms) h m
+               (tot_map_name_inv src) (tot_map_name_inv dst))) =
+    collate_ls name_eq_dec (map tot_map_name ns)
+            (update2 name_eq_dec (fun src dst : name => map tot_map_msg (f (tot_map_name_inv src) (tot_map_name_inv dst)))
+                     (tot_map_name from) (tot_map_name to) (map tot_map_msg ms))
+            (tot_map_name h) (tot_map_msg m).
+Proof.
+move => ns f h m from to ms.
+rewrite -map_msg_update2.
+by rewrite collate_ls_tot_map_eq.
+Qed.
+
+Theorem step_ordered_dynamic_failure_tot_mapped_simulation_1 :
+  forall net net' failed failed' tr,
+    NoDup (odnwNodes net) ->
+    @step_ordered_dynamic_failure _ _ overlay_fst new_msg_fst fail_msg_fst (failed, net) (failed', net') tr ->
+    @step_ordered_dynamic_failure _ _ overlay_snd new_msg_snd fail_msg_snd (map tot_map_name failed, tot_map_odnet net) (map tot_map_name failed', tot_map_odnet net') (map tot_map_trace tr).
+Proof.
+move => net net' failed failed' tr H_nd H_step.
+invcs H_step.
+- rewrite /tot_map_odnet /=.
+  apply (@StepOrderedDynamicFailure_start _ _ _ _ _ _ _ _ (tot_map_name h)) => /=; first exact: not_in_failed_not_in.
+  set p1 := fun _ _ => _.
+  set p2 := collate_ls _ _ _ _ _.
+  set s1 := fun _ => _.
+  set s2 := update _ _ _ _.
+  have H_eq_s: s1 = s2.
+    rewrite /s1 /s2 /update {s1 s2}.
+    apply functional_extensionality => n.
+    rewrite -tot_init_handlers_eq.
+    break_match_goal.
+      break_if; break_if; try by congruence.
+      - by repeat find_rewrite; repeat find_rewrite_lem tot_map_name_inv_inverse.
+      - by find_reverse_rewrite; find_rewrite_lem tot_map_name_inverse_inv.
+      - by find_rewrite.
+    break_if; break_if; (try by congruence); last by find_rewrite.
+    by repeat find_rewrite; repeat find_rewrite_lem tot_map_name_inv_inverse.
+  rewrite H_eq_s /s2 {s1 s2 H_eq_s}.
+  have H_eq_p: p1 = p2.
+    rewrite /p1 /p2 {p1 p2}.
+    rewrite collate_ls_tot_map_eq /=.
+    rewrite collate_tot_map_eq.
+    rewrite tot_new_msg_fst_snd.
+    set f1 := fun _ _ => _.    
+    set c1 := collate _ _ _ _.
+    set c2 := collate _ _ _ _.
+    set f'1 := map tot_map_name _.
+    set f'2 := filter_rel _ (tot_map_name h) _.
+    have H_c: c1 = c2.
+      rewrite /c1 /c2 {c1 c2}.
+      apply: NoDup_Permutation_collate_eq; last first.
+        rewrite /tot_map_name_msgs.
+        by apply: nodup_perm_map_map_pair_perm; last exact: Permutation_refl.
+      rewrite /tot_map_name_msgs /=.
+      apply: NoDup_map_snd_fst => //.
+        apply (@nodup_tot_map msg_new); first exact: in_map2snd_snd.
+        apply: NoDup_map2snd.
+        exact: NoDup_remove_all.
+      move => nm nm' H_in H_in'.
+      apply tot_map_in_snd in H_in.
+      apply tot_map_in_snd in H_in'.
+      by rewrite H_in H_in'.
+    rewrite H_c {H_c}.
+    suff H_suff: f'1 = f'2 by rewrite H_suff.
+    rewrite /f'1 /f'2.
+    elim (odnwNodes net) => /=; first by rewrite 2!remove_all_nil.
+    move => n ns.
+    set mn := tot_map_name n.
+    set mns := map _ ns.
+    set mfailed' := map _ failed'.
+    move => IH.
+    have H_cn := remove_all_cons name_eq_dec failed' n ns.
+    have H_cn' := remove_all_cons name_eq_dec mfailed' mn mns.
+    unfold mn, mns, mfailed' in *.
+    repeat break_or_hyp; repeat break_and; repeat find_rewrite => //=.
+    * by find_apply_lem_hyp not_in_failed_not_in.
+    * by find_apply_lem_hyp in_failed_in.
+    * case adjacent_to_dec => H_dec; case adjacent_to_dec => H_dec' => //=.
+      + by rewrite IH.
+      + by find_apply_lem_hyp tot_adjacent_to_fst_snd.
+      + by find_apply_lem_hyp tot_adjacent_to_fst_snd.
+  by rewrite H_eq_p.
+- rewrite /tot_map_odnet /=.
+  apply (@StepOrderedDynamicFailure_deliver _ _ _ _ _ _ _ _ _ (tot_map_msg m) (map tot_map_msg ms) (map tot_map_output out) (tot_map_data d) (tot_map_data d') (tot_map_name_msgs l) (tot_map_name from) (tot_map_name to)) => //=.
+  * exact: not_in_failed_not_in.
+  * exact: in_failed_in. 
+  * rewrite tot_map_name_inv_inverse.
+    by break_match; congruence.
+  * rewrite 2!tot_map_name_inv_inverse.
+    by find_rewrite.
+  * rewrite -tot_net_handlers_eq /tot_mapped_net_handlers.
+    repeat break_let.
+    by repeat tuple_inversion.
+  * set u1 := fun _ => match _ with | _ => _ end.
+    set u2 := update _ _ _ _.   
+    rewrite collate_tot_map_update2_eq.
+    suff H_suff: u1 = u2 by rewrite H_suff.
+    rewrite /u1 /u2 /update /=.
+    apply functional_extensionality => n.
+    repeat break_if; try by congruence.
+      rewrite -(tot_map_name_inverse_inv n) in n0.
+      by rewrite e in n0.
+    find_rewrite.
+    by find_rewrite_lem tot_map_name_inv_inverse.
+  * by rewrite map_tot_map_trace_eq.
+- rewrite /tot_map_odnet /=.
+  apply (@StepOrderedDynamicFailure_input _ _ _ _ _ (tot_map_name h) _ _ _ _ (map tot_map_output out) (tot_map_input inp) (tot_map_data d) (tot_map_data d') (tot_map_name_msgs l)) => //=.
+  * exact: not_in_failed_not_in.
+  * exact: in_failed_in. 
+  * rewrite tot_map_name_inv_inverse.
+    by break_match; congruence.
+  * rewrite /= -tot_input_handlers_eq /tot_mapped_input_handlers.
+    repeat break_let.
+    by repeat tuple_inversion.
+  * rewrite collate_tot_map_eq.
+    set u1 := fun _ => match _ with | _ => _ end.
+    set u2 := update _ _ _ _.   
+    suff H_suff: u1 = u2 by rewrite H_suff.
+    rewrite /u1 /u2 /update /=.
+    apply functional_extensionality => n.
+    repeat break_if; try by congruence.
+      rewrite -(tot_map_name_inverse_inv n) in n0.
+      by rewrite e in n0.
+    find_rewrite.
+    by find_rewrite_lem tot_map_name_inv_inverse.
+  * by rewrite map_tot_map_trace_eq.
+- rewrite /tot_map_odnet /=.  
+  set l := map2snd _ _.
+  have H_nd': NoDup (map (fun nm => fst nm) (tot_map_name_msgs l)).
+    rewrite /tot_map_name_msgs /=.
+    rewrite /l {l}.
+    apply NoDup_map_snd_fst.
+      apply (@nodup_tot_map msg_fail); first exact: in_map2snd_snd.
+      apply NoDup_map2snd.
+      exact: NoDup_remove_all.
+    move => nm nm' H_in H_in'.
+    have H_fail := tot_map_in_snd _ _ _ _ H_in.
+    have H_fail' := tot_map_in_snd _ _ _ _ H_in'.
+    by rewrite H_fail H_fail'.
+  have H_pm := map_msg_fail_eq_nodup h failed H_nd (Permutation_refl (map tot_map_name (odnwNodes net))).
+  have H_eq := NoDup_Permutation_collate_eq  _ _ name_eq_dec _ _ _ _ H_nd' H_pm.
+  rewrite /l /tot_map_name_msgs in H_eq.
+  apply: StepOrderedDynamicFailure_fail.
+  * exact: not_in_failed_not_in.
+  * exact: in_failed_in. 
+  * rewrite /=.
+    rewrite /l collate_tot_map_eq /tot_map_name_msgs.
+    by rewrite H_eq.
+Qed.
+
+Corollary step_ordered_dynamic_failure_tot_mapped_simulation_star_1 :
+  forall net failed tr,
+    @step_ordered_dynamic_failure_star _ _ overlay_fst new_msg_fst fail_msg_fst step_ordered_dynamic_failure_init (failed, net) tr ->
+    @step_ordered_dynamic_failure_star _ _ overlay_snd new_msg_snd fail_msg_snd step_ordered_dynamic_failure_init (map tot_map_name failed, tot_map_odnet net) (map tot_map_trace tr).
+Proof.
+move => net failed tr H_step.
+remember step_ordered_dynamic_failure_init as y in *.
+change failed with (fst (failed, net)).
+change net with (snd (failed, net)) at 2.
+move: Heqy.
+induction H_step using refl_trans_1n_trace_n1_ind => H_init /=.
+  rewrite H_init /step_ordered_dynamic_failure_init /= /step_ordered_failure_init.
+  exact: RT1nTBase.
+concludes.
+repeat find_rewrite.
+destruct x'.
+destruct x''.
+rewrite /=.
+find_apply_lem_hyp step_ordered_dynamic_failure_tot_mapped_simulation_1.
+  rewrite map_app.
+  match goal with
+  | H : step_ordered_dynamic_failure_star _ _ _ |- _ => apply: (refl_trans_1n_trace_trans H)
+  end.
+  rewrite (app_nil_end (map tot_map_trace _)).
+  apply (@RT1nTStep _ _ _ _ (map tot_map_name l0, tot_map_odnet o0)) => //.
+  exact: RT1nTBase.
+move: H_step1.
+exact: ordered_dynamic_nodes_no_dup.
 Qed.
 
 End TotalMapSimulations.
