core/DynamicNetLemmas.v
@@ -1,0 +1,224 @@
+Require Import Verdi.Verdi.
+
+Require Import StructTact.Update.
+Require Import FunctionalExtensionality.
+Require Import Sumbool.
+Require Import Relation_Definitions.
+Require Import RelationClasses.
+
+Require Import mathcomp.ssreflect.ssreflect.
+
+Set Implicit Arguments.
+
+Section DynamicNetLemmas.
+
+Context {base_params : BaseParams}.
+Context {multi_params : MultiParams base_params}.
+Context {overlay_params : NameOverlayParams multi_params}.
+Context {new_msg_params : NewMsgParams multi_params}.
+Context {fail_msg_params : FailMsgParams multi_params}.
+
+Lemma ordered_dynamic_uninitialized_state :
+forall net failed tr,
+ step_ordered_dynamic_failure_star step_ordered_dynamic_failure_init (failed, net) tr ->
+ forall n, ~ In n (odnwNodes net) ->
+ odnwState net n = None.
+Proof.
+move => net failed tr H.
+remember step_ordered_dynamic_failure_init as y in *.
+have ->: net = snd (failed, net) by [].
+move: Heqy.
+induction H using refl_trans_1n_trace_n1_ind => H_init /=; first by rewrite H_init.
+concludes => {H_init}.
+match goal with
+| [ H : step_ordered_dynamic_failure _ _ _ |- _ ] => invc H
+end; rewrite /=.
+- move => n H_in.
+  rewrite /= in IHrefl_trans_1n_trace1.
+  rewrite /update /=.
+  have H_neq: h <> n by move => H_eq; case: H_in; left.
+  have H_not_in: ~ In n (odnwNodes net0) by move => H_not_in; case: H_in; right.
+  case name_eq_dec => H_dec; first by rewrite H_dec in H_neq.
+  exact: IHrefl_trans_1n_trace1.
+- move => n H_in.
+  rewrite /= in IHrefl_trans_1n_trace1.
+  rewrite /update /=.
+  have H_neq: n <> to by move => H_eq; rewrite H_eq in H_in.
+  case name_eq_dec => H_dec //.
+  exact: IHrefl_trans_1n_trace1.
+- move => n H_in.
+  rewrite /= in IHrefl_trans_1n_trace1.
+  rewrite /update.
+  have H_neq: n <> h by move => H_eq; rewrite H_eq in H_in.
+  case name_eq_dec => H_dec //.
+  exact: IHrefl_trans_1n_trace1.
+- move => n H_in.
+  rewrite /= in IHrefl_trans_1n_trace1.
+  exact: IHrefl_trans_1n_trace1.
+Qed.
+
+Lemma ordered_dynamic_initialized_state :
+forall net failed tr,
+ step_ordered_dynamic_failure_star step_ordered_dynamic_failure_init (failed, net) tr ->
+ forall n, In n (odnwNodes net) ->
+ exists d, odnwState net n = Some d.
+Proof.
+move => net failed tr H.
+remember step_ordered_dynamic_failure_init as y in *.
+have ->: net = snd (failed, net) by [].
+move: Heqy.
+induction H using refl_trans_1n_trace_n1_ind => H_init /=; first by rewrite H_init.
+repeat find_rewrite.
+concludes => {H_init}.
+match goal with
+| [ H : step_ordered_dynamic_failure _ _ _ |- _ ] => invc H
+end; rewrite /=.
+- move => n H_in.
+  case: H_in => H_in.
+    rewrite -H_in /update.
+    break_if => //.
+    by exists (init_handlers h).
+  have H_neq: n <> h by move => H_eq; rewrite H_eq in H_in.
+  have [d H_eq] := IHrefl_trans_1n_trace1 _ H_in.
+  exists d.
+  rewrite /update /=.
+  by break_if.
+- move => n H_in.
+  rewrite /update.
+  break_if; first by exists d'.
+  have [d0 H_eq] := IHrefl_trans_1n_trace1 _ H_in.
+  by exists d0.
+- move => n H_in.
+  rewrite /update.
+  break_if; first by exists d'.
+  have [d0 H_eq] := IHrefl_trans_1n_trace1 _ H_in.
+  by exists d0.
+- move => n H_in.
+  exact: IHrefl_trans_1n_trace1.
+Qed.
+
+Lemma ordered_dynamic_failed_then_initialized :
+forall net failed tr,
+ step_ordered_dynamic_failure_star step_ordered_dynamic_failure_init (failed, net) tr ->
+ forall n, In n failed ->
+ In n (odnwNodes net).
+Proof.
+move => net failed tr H.
+remember step_ordered_dynamic_failure_init as y in *.
+have ->: failed = fst (failed, net) by [].
+have H_eq_o: net = snd (failed, net) by [].
+rewrite {2}H_eq_o {H_eq_o}.
+move: Heqy.
+induction H using refl_trans_1n_trace_n1_ind => H_init /=; first by rewrite H_init.
+repeat find_rewrite.
+concludes => {H_init}.
+match goal with
+| [ H : step_ordered_dynamic_failure _ _ _ |- _ ] => invc H
+end; rewrite /=.
+- move => n H_in.
+  right.
+  exact: IHrefl_trans_1n_trace1.
+- move => n H_in.
+  exact: IHrefl_trans_1n_trace1.
+- move => n H_in.
+  exact: IHrefl_trans_1n_trace1.
+- move => n H_in.
+  case: H_in => H_in; first by rewrite -H_in.
+  exact: IHrefl_trans_1n_trace1.
+Qed.
+
+Lemma ordered_dynamic_state_not_initialized_not_failed : 
+forall net failed tr,
+ step_ordered_dynamic_failure_star step_ordered_dynamic_failure_init (failed, net) tr ->
+ forall n, ~ In n (odnwNodes net) ->
+ ~ In n failed.
+Proof.
+move => net failed tr H.
+remember step_ordered_dynamic_failure_init as y in *.
+have ->: failed = fst (failed, net) by [].
+have H_eq_o: net = snd (failed, net) by [].
+rewrite {1}H_eq_o {H_eq_o}.
+move: Heqy.
+induction H using refl_trans_1n_trace_n1_ind => H_init /=; first by rewrite H_init.
+repeat find_rewrite.
+concludes => {H_init}.
+match goal with
+| [ H : step_ordered_dynamic_failure _ _ _ |- _ ] => invc H
+end; rewrite /=.
+- move => n H_in.
+  have H_not_in: ~ In n (odnwNodes net0) by move => H_in'; case: H_in; right.
+  exact: IHrefl_trans_1n_trace1.
+- move => n H_in.
+  exact: IHrefl_trans_1n_trace1.
+- move => n H_in.
+  exact: IHrefl_trans_1n_trace1.
+- move => n H_in.
+  move => H_or.
+  case: H_or => H_or; first by repeat find_rewrite.
+  contradict H_or.
+  exact: IHrefl_trans_1n_trace1.
+Qed.
+
+Lemma ordered_dynamic_no_outgoing_uninitialized :
+forall onet failed tr,
+  step_ordered_dynamic_failure_star step_ordered_dynamic_failure_init (failed, onet) tr -> 
+  forall n, ~ In n (odnwNodes onet) ->
+  forall n', onet.(odnwPackets) n n' = [].
+Proof.
+move => net failed tr H.
+remember step_ordered_dynamic_failure_init as y in *.
+have ->: net = snd (failed, net) by [].
+move: Heqy.
+induction H using refl_trans_1n_trace_n1_ind => H_init /=; first by rewrite H_init.
+concludes => {H_init}.
+match goal with
+| [ H : step_ordered_dynamic_failure _ _ _ |- _ ] => invc H
+end; rewrite /=.
+- move => n H_a n'. 
+  have H_neq: h <> n by eauto.
+  have H_not_in: ~ In n (odnwNodes net0) by eauto.
+  rewrite collate_ls_not_in; first by rewrite collate_neq //; eauto.
+  apply: not_in_not_in_filter_rel.
+  move => H_in.
+  case: H_not_in.
+  move: H_in.
+  exact: in_remove_all_was_in.
+- move => n H_a n'.
+  have H_neq: to <> n by move => H_eq; rewrite -H_eq in H_a.
+  rewrite collate_neq //.
+  rewrite /update2.
+  case sumbool_and => H_and; last by eauto.
+  break_and; repeat find_rewrite.
+  simpl in *.
+  have IH := IHrefl_trans_1n_trace1 _ H_a.
+  by find_higher_order_rewrite.
+- move => n H_a n'.
+  have H_neq: h <> n by move => H_eq; rewrite -H_eq in H_a.
+  rewrite collate_neq //.
+  by eauto.
+- move => n H_a n'.
+  have H_neq: h <> n by move => H_eq; rewrite -H_eq in H_a.
+  rewrite collate_neq //.
+  by eauto.
+Qed.
+
+Lemma ordered_dynamic_nodes_no_dup :
+forall onet failed tr,
+  step_ordered_dynamic_failure_star step_ordered_dynamic_failure_init (failed, onet) tr -> 
+  NoDup (odnwNodes onet).
+Proof.
+move => net failed tr H.
+remember step_ordered_dynamic_failure_init as y in *.
+have ->: net = snd (failed, net) by [].
+move: Heqy.
+induction H using refl_trans_1n_trace_n1_ind => H_init.
+  rewrite H_init /=.
+  exact: NoDup_nil.
+concludes => {H_init}.
+match goal with
+| [ H : step_ordered_dynamic_failure _ _ _ |- _ ] => invc H
+end; rewrite //=.
+exact: NoDup_cons.
+Qed.
+
+End DynamicNetLemmas.
